Part 1:

1. Proof by Contradiction
sqrt(2) = irrational\
sqrt(2) = 1.41\
w=p/q

2. Proof by Exhaustion\
sqrt(25) = 5 | 5+5 = 10\
sqrt(100) = 10 | 10+10 = 20\
sqrt(169) = 13 | 13+13 = 26\
False.

3. Direct Proof\
(2n+1)+(2m+1)\
2n+2m+2\
2(n+m+1)\
let p = n+m+1\
2p\
True.

4. even = (2n)+ n^2\
Direct Proof
2n+1 + 2n+1 = 2n\
4n+2 = 2n\
Even

5. n^2 = odd, then n = odd\
Contraposition\
n^2 = even, n = even\
n = 2k\
(2k)^2\
4k^2 = even\

Part 2:

1. 1 + 5 + 9 + ... + (4n-3) = n(2n-1)\
Base case:\
n(2n-1)\
1(2(1)-1) = 1\
1 = 1 \
True.\
Inductive Hypothesis:\
1+5+9+...+(4n-3)+(4(n+1)-3) = n(2n-1)\
n(2n-1)+(4(n+1)-3) = (n+1)(2(n+1)-1)\
2n^2-n+4n+1 = (n+1)(2n+1)\
2n^2+3n+1 = 2n^2+3n+1

2.1+2+3+...+n = (n^3+2n)/3\
Base Case:\
1=(1^3+2(1))/3
1=1\
True.\
Inductive Hypothesis:\
1+2+3+...+n+(n+1) = (n^3+2n)/3
(n^3+2n)/3 + (n+1) = ((n+1)^3+2(n+1))/3
3n^3+6n+n+1 = (n^3+3n^2+3n+1+2n+2)/3
3n^3+7n+1 = (n^3+3n^2+5n+3)/3

3. n>= 1, 9^n-1 is divisible by 8
Base case:\
9^1-1\
8/8\
1 = 1\
Inductive Hypothesis:\
(9^(k+1)-1)\
(8m+1)* 9-1\
72m+9\
8(9m+1)\
Divisible by 8.
